src/Lean/Elab/Tactic/Try.lean
@@ -33,6 +33,12 @@ private def addSuggestion (stx : TryThis.Suggestion) : M Bool := do
   TryThis.addSuggestion (← read).tk stx (origSpan? := (← getRef))
   return true
 
+-- TODO: vanilla `induction`.
+-- TODO: cleanup the whole file, and use better combinators
+-- TODO: make it extensible.
+-- TODO: librarySearch integration.
+-- TODO: premise selection.
+
 private def failed (msg : MessageData) : M Bool := do
   trace[«try»] msg
   return false
@@ -62,39 +68,81 @@ private def collect : M Try.Info := do
 private def toIdent (declName : Name) : MetaM Ident := do
   return mkIdent (← unresolveNameGlobalAvoidingLocals declName)
 
-inductive GrindKind where
-  | tactic
+inductive TacticKind where
+  | exec
   | suggestion
-  | errorMsg
+  | error
 
-private def mkGrindStx (params : Array (TSyntax ``Parser.Tactic.grindParam)) (kind : GrindKind := .tactic) : MetaM (TSyntax `tactic) := do
+private def mkGrindStx (params : Array (TSyntax ``Parser.Tactic.grindParam)) (kind : TacticKind) : MetaM (TSyntax `tactic) := do
   let result ← match kind with
-    | .tactic => `(tactic| grind -verbose)
+    | .exec => `(tactic| grind -verbose)
     | .suggestion => `(tactic| grind?)
-    | .errorMsg => `(tactic| grind)
-  let paramsStx := #[mkAtom "[", (mkAtom ",").mkSep params, mkAtom "]"]
-  return ⟨result.raw.setArg 3 (mkNullNode paramsStx)⟩
+    | .error => `(tactic| grind)
+  if params.isEmpty then
+    return result
+  else
+    let paramsStx := #[mkAtom "[", (mkAtom ",").mkSep params, mkAtom "]"]
+    return ⟨result.raw.setArg 3 (mkNullNode paramsStx)⟩
 
-private def tryGrindWith (params : Array (TSyntax ``Parser.Tactic.grindParam)) : M Bool := do
-  let stx ← mkGrindStx params
-  (do
-    evalTactic stx
-    addSuggestion (← mkGrindStx params .suggestion))
-  <|>
-  (do failed m!"`{← mkGrindStx params .errorMsg}` failed")
-
-private def tryGrindEqnsCore (declNames : Std.HashSet Name) : M Bool := do
-  if declNames.isEmpty then return false
+private def mkGrindEqnsStx (declNames : Std.HashSet Name) : M (TacticKind → MetaM (TSyntax `tactic)) := do
   let mut params := #[]
   for declName in declNames do
     params := params.push (← `(Parser.Tactic.grindParam| = $(← toIdent declName)))
-  tryGrindWith params
+  return mkGrindStx params
+
+private def tryTac' (mkTac : TacticKind → MetaM (TSyntax `tactic)) : M Bool := do
+  let stx ← mkTac .exec
+  (do
+    focusAndDone <| evalTactic stx
+    addSuggestion (← mkTac .suggestion))
+  <|>
+  (do failed m!"`{← mkTac .error}` failed")
 
 private def tryGrindEqns (info : Try.Info) : M Bool := do
-  tryGrindEqnsCore info.eqnCandidates
+  if info.eqnCandidates.isEmpty then return false
+  tryTac' (← mkGrindEqnsStx info.eqnCandidates)
 
 private def tryGrindUnfold (info : Try.Info) : M Bool := do
-  tryGrindEqnsCore info.unfoldCandidates
+  if info.unfoldCandidates.isEmpty then return false
+  tryTac' (← mkGrindEqnsStx info.unfoldCandidates)
+
+private def allAccessible (majors : Array FVarId) : MetaM Bool :=
+  majors.allM fun major => do
+    let localDecl ← major.getDecl
+    -- TODO: we are not checking shadowed variables
+    return !localDecl.userName.hasMacroScopes
+
+open Try.Collector in
+private partial def tryFunIndsCore (info : Try.Info) (mkBody : TacticKind → MetaM (TSyntax `tactic)) : M Bool := do
+  go info.funIndCandidates.toList
+where
+  go' (c : FunIndCandidate) : M Bool := do
+    if (← allAccessible c.majors) then
+      let mut terms := #[]
+      for major in c.majors do
+        let localDecl ← major.getDecl
+        terms := terms.push (← `($(mkIdent localDecl.userName):term))
+      let indFn ← toIdent c.funIndDeclName
+      tryTac' fun k => do
+        let body ← mkBody k
+        `(tactic| induction $terms,* using $indFn <;> $body)
+    else
+      -- TODO: use `rename_i`
+      failed "`induction` failed, majors contain inaccessible vars {c.majors.map mkFVar}"
+
+  go (cs : List FunIndCandidate) : M Bool := do
+    match cs with
+    | [] => return false
+    | c::cs =>
+      trace[try.debug.funInd] "{c.funIndDeclName}, {c.majors.map mkFVar}"
+      go' c <||> go cs
+
+private partial def tryFunIndsGrind (info : Try.Info) : M Bool :=
+  tryFunIndsCore info (mkGrindStx #[])
+
+private partial def tryFunIndsGrindEqns (info : Try.Info) : M Bool := do
+  if info.eqnCandidates.isEmpty then return false
+  tryFunIndsCore info (← mkGrindEqnsStx info.eqnCandidates)
 
 private def evalTryTraceCore : M Unit := do
   if (← trySimp) then return ()
@@ -103,6 +151,8 @@ private def evalTryTraceCore : M Unit := do
   let info ← collect
   if (← tryGrindEqns info) then return ()
   if (← tryGrindUnfold info) then return ()
+  if (← tryFunIndsGrind info) then return ()
+  if (← tryFunIndsGrindEqns info) then return ()
   Meta.throwTacticEx `«try?» (← read).mvarId "consider using `grind` manually, `set_option trace.try true` shows everything `try?` tried"
 
 @[builtin_tactic Lean.Parser.Tactic.tryTrace] def evalTryTrace : Tactic := fun stx => do
