src/Lean/Meta/Tactic/Try.lean
@@ -12,4 +12,6 @@ builtin_initialize registerTraceClass `try
 builtin_initialize registerTraceClass `try.collect
 builtin_initialize registerTraceClass `try.collect.funInd
 
+builtin_initialize registerTraceClass `try.debug.funInd
+
 end Lean
